correctness/RegexCorrectness/NFA/Semantics/Equivalence/CapturesOfPath.lean
@@ -7,18 +7,19 @@ set_option autoImplicit false
 namespace Regex.NFA
 
 open Regex.Data (Expr)
+open String (ValidPos)
 
-variable {nfa : NFA} {next e result it it' update}
+variable {s : String} {nfa : NFA} {next e result} {pos pos' : ValidPos s} {update}
 
 theorem captures_of_path.group {tag} (eq : nfa.pushRegex next (.group tag e) = result)
   (wf : nfa.WellFormed) (next_lt : next < nfa.nodes.size)
-  (path : result.Path nfa.nodes.size result.start it next it' update)
-  (ih : ∀ {nfa : NFA} {next result it it' update}, nfa.pushRegex next e = result →
+  (path : result.Path nfa.nodes.size result.start pos next pos' update)
+  (ih : ∀ {nfa : NFA} {next result} {pos pos' : ValidPos s} {update}, nfa.pushRegex next e = result →
     nfa.WellFormed →
     next < nfa.nodes.size →
-    result.Path nfa.nodes.size result.start it next it' update →
-    ∃ groups, EquivUpdate groups update ∧ e.Captures it it' groups) :
-  ∃ groups, EquivUpdate groups update ∧ (Expr.group tag e).Captures it it' groups := by
+    result.Path nfa.nodes.size result.start pos next pos' update →
+    ∃ groups, EquivUpdate groups update ∧ e.Captures pos pos' groups) :
+  ∃ groups, EquivUpdate groups update ∧ (Expr.group tag e).Captures pos pos' groups := by
   open Compile.ProofData Group in
   let pd := Group.intro eq
   simp [pd.eq_result eq] at path
@@ -56,7 +57,7 @@ theorem captures_of_path.group {tag} (eq : nfa.pushRegex next (.group tag e) = r
       have ⟨_, hit, hupdate⟩ := step_close_iff.mp (step.cast this)
       rw [←hit] at c
       simp [equ, hupdate, ←hit]
-      exact ⟨.group tag it.pos it'.pos groupExpr, .group eqv, .group c⟩
+      exact ⟨.group tag pos pos' groupExpr, .group eqv, .group c⟩
     | more step rest =>
       have ⟨hj, _, _⟩ := step_close_iff.mp (step.cast this)
       have : nfa.nodes.size ≤ next := show nfa.nodes.size ≤ pd.next from hj ▸ rest.ge
@@ -64,18 +65,18 @@ theorem captures_of_path.group {tag} (eq : nfa.pushRegex next (.group tag e) = r
 
 theorem captures_of_path.alternate {e₁ e₂} (eq : nfa.pushRegex next (.alternate e₁ e₂) = result)
   (wf : nfa.WellFormed) (next_lt : next < nfa.nodes.size)
-  (path : result.Path nfa.nodes.size result.start it next it' update)
-  (ih₁ : ∀ {nfa : NFA} {next result it it' update}, nfa.pushRegex next e₁ = result →
+  (path : result.Path nfa.nodes.size result.start pos next pos' update)
+  (ih₁ : ∀ {nfa : NFA} {next result} {pos pos' : ValidPos s} {update}, nfa.pushRegex next e₁ = result →
     nfa.WellFormed →
     next < nfa.nodes.size →
-    result.Path nfa.nodes.size result.start it next it' update →
-    ∃ groups, EquivUpdate groups update ∧ e₁.Captures it it' groups)
-  (ih₂ : ∀ {nfa : NFA} {next result it it' update}, nfa.pushRegex next e₂ = result →
+    result.Path nfa.nodes.size result.start pos next pos' update →
+    ∃ groups, EquivUpdate groups update ∧ e₁.Captures pos pos' groups)
+  (ih₂ : ∀ {nfa : NFA} {next result} {pos pos' : ValidPos s} {update}, nfa.pushRegex next e₂ = result →
     nfa.WellFormed →
     next < nfa.nodes.size →
-    result.Path nfa.nodes.size result.start it next it' update →
-    ∃ groups, EquivUpdate groups update ∧ e₂.Captures it it' groups) :
-  ∃ groups, EquivUpdate groups update ∧ (Expr.alternate e₁ e₂).Captures it it' groups := by
+    result.Path nfa.nodes.size result.start pos next pos' update →
+    ∃ groups, EquivUpdate groups update ∧ e₂.Captures pos pos' groups) :
+  ∃ groups, EquivUpdate groups update ∧ (Expr.alternate e₁ e₂).Captures pos pos' groups := by
   open Compile.ProofData Alternate in
   let pd := Alternate.intro eq
   simp [pd.eq_result eq] at path
@@ -99,7 +100,7 @@ theorem captures_of_path.alternate {e₁ e₂} (eq : nfa.pushRegex next (.altern
       simp [hj, hit] at rest
 
       have rest := castTo₂ wf next_lt rest
-      have rest : nfa₂.Path nfa₁.nodes.size nfa₂.start it next it' updates := by
+      have rest : nfa₂.Path nfa₁.nodes.size nfa₂.start pos next pos' updates := by
         apply rest.liftBound' (ge_pushRegex_start rfl)
         intro i it j it' update gei gej step
         cases (step.liftBound' gei).eq_or_ge_of_pushRegex with
@@ -114,18 +115,18 @@ theorem captures_of_path.alternate {e₁ e₂} (eq : nfa.pushRegex next (.altern
 
 theorem captures_of_path.concat {e₁ e₂} (eq : nfa.pushRegex next (.concat e₁ e₂) = result)
   (wf : nfa.WellFormed) (next_lt : next < nfa.nodes.size)
-  (path : result.Path nfa.nodes.size result.start it next it' update)
-  (ih₁ : ∀ {nfa : NFA} {next result it it' update}, nfa.pushRegex next e₁ = result →
+  (path : result.Path nfa.nodes.size result.start pos next pos' update)
+  (ih₁ : ∀ {nfa : NFA} {next result} {pos pos' : ValidPos s} {update}, nfa.pushRegex next e₁ = result →
     nfa.WellFormed →
     next < nfa.nodes.size →
-    result.Path nfa.nodes.size result.start it next it' update →
-    ∃ groups, EquivUpdate groups update ∧ e₁.Captures it it' groups)
-  (ih₂ : ∀ {nfa : NFA} {next result it it' update}, nfa.pushRegex next e₂ = result →
+    result.Path nfa.nodes.size result.start pos next pos' update →
+    ∃ groups, EquivUpdate groups update ∧ e₁.Captures pos pos' groups)
+  (ih₂ : ∀ {nfa : NFA} {next result} {pos pos' : ValidPos s} {update}, nfa.pushRegex next e₂ = result →
     nfa.WellFormed →
     next < nfa.nodes.size →
-    result.Path nfa.nodes.size result.start it next it' update →
-    ∃ groups, EquivUpdate groups update ∧ e₂.Captures it it' groups) :
-  ∃ groups, EquivUpdate groups update ∧ (Expr.concat e₁ e₂).Captures it it' groups := by
+    result.Path nfa.nodes.size result.start pos next pos' update →
+    ∃ groups, EquivUpdate groups update ∧ e₂.Captures pos pos' groups) :
+  ∃ groups, EquivUpdate groups update ∧ (Expr.concat e₁ e₂).Captures pos pos' groups := by
   open Compile.ProofData Concat in
   let pd := Concat.intro eq
   simp [pd.eq_result eq] at path
@@ -140,13 +141,13 @@ theorem captures_of_path.concat {e₁ e₂} (eq : nfa.pushRegex next (.concat e�
   exact ⟨.concat group₁ group₂, equ ▸ .concat eqv₁ eqv₂, .concat c₁ c₂⟩
 
 open Compile.ProofData Star in
-theorem captures_of_path.star_of_loop [Star] {greedy} (loop : Loop it it' update)
-  (ih : ∀ {it it' update},
-    nfa'.Path nfaPlaceholder.nodes.size nfaExpr.start it nfaPlaceholder.start it' update →
-    ∃ groups, EquivUpdate groups update ∧ e.Captures it it' groups) :
-  ∃ groups, EquivUpdate groups update ∧ (Expr.star greedy e).Captures it it' groups := by
+theorem captures_of_path.star_of_loop [Star] {greedy} (loop : Loop pos pos' update)
+  (ih : ∀ {pos pos' : ValidPos s} {update},
+    nfa'.Path nfaPlaceholder.nodes.size nfaExpr.start pos nfaPlaceholder.start pos' update →
+    ∃ groups, EquivUpdate groups update ∧ e.Captures pos pos' groups) :
+  ∃ groups, EquivUpdate groups update ∧ (Expr.star greedy e).Captures pos pos' groups := by
   induction loop with
-  | last step => exact ⟨.empty, .empty, .starEpsilon step.validL⟩
+  | last step => exact ⟨.empty, .empty, .starEpsilon⟩
   | loop pathExpr _ ihLoop =>
     have ⟨groups₁, eqv₁, c₁⟩ := ih pathExpr
     have ⟨groups₂, eqv₂, c₂⟩ := ihLoop
@@ -154,13 +155,13 @@ theorem captures_of_path.star_of_loop [Star] {greedy} (loop : Loop it it' update
 
 theorem captures_of_path.star {greedy e} (eq : nfa.pushRegex next (.star greedy e) = result)
   (wf : nfa.WellFormed) (next_lt : next < nfa.nodes.size)
-  (path : result.Path nfa.nodes.size result.start it next it' update)
-  (ih : ∀ {nfa : NFA} {next result it it' update}, nfa.pushRegex next e = result →
+  (path : result.Path nfa.nodes.size result.start pos next pos' update)
+  (ih : ∀ {nfa : NFA} {next result} {pos pos' : ValidPos s} {update}, nfa.pushRegex next e = result →
     nfa.WellFormed →
     next < nfa.nodes.size →
-    result.Path nfa.nodes.size result.start it next it' update →
-    ∃ groups, EquivUpdate groups update ∧ e.Captures it it' groups) :
-  ∃ groups, EquivUpdate groups update ∧ (Expr.star greedy e).Captures it it' groups := by
+    result.Path nfa.nodes.size result.start pos next pos' update →
+    ∃ groups, EquivUpdate groups update ∧ e.Captures pos pos' groups) :
+  ∃ groups, EquivUpdate groups update ∧ (Expr.star greedy e).Captures pos pos' groups := by
   open Compile.ProofData Star in
   let pd := Star.intro eq
   simp [pd.eq_result eq] at path
@@ -174,10 +175,10 @@ theorem captures_of_path.star {greedy e} (eq : nfa.pushRegex next (.star greedy 
 
 theorem captures_of_path (eq : nfa.pushRegex next e = result)
   (wf : nfa.WellFormed) (next_lt : next < nfa.nodes.size)
-  (path : result.Path nfa.nodes.size result.start it next it' update) :
-  ∃ groups, EquivUpdate groups update ∧ e.Captures it it' groups := by
+  (path : result.Path nfa.nodes.size result.start pos next pos' update) :
+  ∃ groups, EquivUpdate groups update ∧ e.Captures pos pos' groups := by
   open Compile.ProofData in
-  induction e generalizing nfa next result it it' update with
+  induction e generalizing nfa next result pos pos' update with
   | empty =>
     let pd := Empty.intro eq
     simp [pd.eq_result eq] at path
@@ -187,32 +188,29 @@ theorem captures_of_path (eq : nfa.pushRegex next e = result)
     simp [pd.eq_result eq] at path
     have := (pd.path_start_iff next_lt).mp path
     simp [this]
-    exact ⟨.empty, .empty, .epsilon (by simp [this])⟩
+    exact ⟨.empty, .empty, .epsilon⟩
   | anchor a =>
     let pd := Anchor.intro eq
     simp [pd.eq_result eq] at path
-    have ⟨_, eqs, equ, v, test⟩:= (pd.path_start_iff next_lt).mp path
-    simp [eqs, equ]
-    exact ⟨.empty, .empty, .anchor v test⟩
+    obtain ⟨_, rfl, rfl, test⟩:= (pd.path_start_iff next_lt).mp path
+    exact ⟨.empty, .empty, .anchor test⟩
   | char c =>
     let pd := Char.intro eq
     simp [pd.eq_result eq] at path
-    have ⟨r, eqr, eqn, eqit, equpdate, vf⟩ := (pd.path_start_iff next_lt).mp path
-    simp [eqit, equpdate]
-    exact ⟨.empty, .empty, .char vf⟩
+    obtain ⟨_, rfl, ne, rfl, rfl⟩ := (pd.path_start_iff next_lt).mp path
+    exact ⟨.empty, .empty, .char ne rfl⟩
   | classes cs =>
     let pd := Classes.intro eq
     simp [pd.eq_result eq] at path
-    have ⟨l, c, r, eqn, eqit, equpdate, vf, mem⟩ := (pd.path_start_iff next_lt).mp path
-    simp [eqit, equpdate]
-    exact ⟨.empty, .empty, .sparse vf mem⟩
+    obtain ⟨_, rfl, ne, rfl, mem⟩ := (pd.path_start_iff next_lt).mp path
+    exact ⟨.empty, .empty, .sparse ne mem⟩
   | group tag e ih => exact captures_of_path.group eq wf next_lt path ih
   | alternate e₁ e₂ ih₁ ih₂ => exact captures_of_path.alternate eq wf next_lt path ih₁ ih₂
   | concat e₁ e₂ ih₁ ih₂ => exact captures_of_path.concat eq wf next_lt path ih₁ ih₂
   | star greedy e ih => exact captures_of_path.star eq wf next_lt path ih
 
-theorem captures_of_path_compile (eq : compile e = nfa) (path : nfa.Path 1 nfa.start it 0 it' update) :
-  ∃ groups, EquivUpdate groups update ∧ e.Captures it it' groups := by
+theorem captures_of_path_compile (eq : compile e = nfa) (path : nfa.Path 1 nfa.start pos 0 pos' update) :
+  ∃ groups, EquivUpdate groups update ∧ e.Captures pos pos' groups := by
   simp [←eq, compile] at path
   exact captures_of_path rfl done_WellFormed (by decide) path
 
