correctness/RegexCorrectness/NFA/Semantics/Equivalence/PathOfCaptures.lean
@@ -6,45 +6,46 @@ set_option autoImplicit false
 
 namespace Regex.NFA
 
-open Regex.Data (Expr)
+open Regex.Data (Expr CaptureGroups)
+open String (ValidPos)
 
-variable {nfa : NFA} {next e result it it' groups}
+variable {s : String} {nfa : NFA} {next e result} {pos pos' : ValidPos s} {groups : CaptureGroups s}
 
 theorem path_of_captures.group {tag} (eq : nfa.pushRegex next (.group tag e) = result)
-  (wf : nfa.WellFormed) (next_lt : next < nfa.nodes.size) (v : it.Valid) (v' : it'.Valid)
+  (wf : nfa.WellFormed) (next_lt : next < nfa.nodes.size)
   (ih : ∀ {nfa : NFA} {next result}, nfa.pushRegex next e = result →
     nfa.WellFormed →
     next < nfa.nodes.size →
-    ∃ update, EquivUpdate groups update ∧ result.Path nfa.nodes.size result.start it next it' update) :
-  ∃ update, EquivUpdate (.group tag it.pos it'.pos groups) update ∧ result.Path nfa.nodes.size result.start it next it' update := by
+    ∃ update, EquivUpdate groups update ∧ result.Path nfa.nodes.size result.start pos next pos' update) :
+  ∃ update, EquivUpdate (.group tag pos pos' groups) update ∧ result.Path nfa.nodes.size result.start pos next pos' update := by
   open Compile.ProofData Group in
   let pd := Group.intro eq
   simp [eq_result eq]
 
   have wf_close := wf_close wf next_lt
   have ⟨update, eqv, path⟩ := ih (result := nfaExpr) rfl wf_close wf_close.start_lt
-  exists (2 * tag, it.pos) :: update ++ [(2 * tag + 1, it'.pos)], .group eqv
+  exists (2 * tag, pos) :: update ++ [(2 * tag + 1, pos')], .group eqv
 
-  have stepOpen : nfa'.Step nfa.nodes.size nfa'.start it nfaExpr.start it (.some (2 * tag, it.pos)) := by
+  have stepOpen : nfa'.Step nfa.nodes.size nfa'.start pos nfaExpr.start pos (.some (2 * tag, pos)) := by
     apply step_start_iff.mpr
-    exact ⟨rfl, rfl, rfl, v⟩
+    exact ⟨rfl, rfl, rfl⟩
   have path := castFromExpr path
-  have path : nfa'.Path nfa.nodes.size nfaExpr.start it nfaClose.start it' update :=
+  have path : nfa'.Path nfa.nodes.size nfaExpr.start pos nfaClose.start pos' update :=
     path.liftBound (by simp [Group.nfaClose]; exact Nat.le_succ _)
-  have pathClose : nfa'.Path nfa.nodes.size nfaClose.start it' next it' [(2 * tag + 1, it'.pos)] := by
-    have stepClose : nfa'.Step nfa.nodes.size nfaClose.start it' next it' (.some (2 * tag + 1, it'.pos)) := by
+  have pathClose : nfa'.Path nfa.nodes.size nfaClose.start pos' next pos' [(2 * tag + 1, pos')] := by
+    have stepClose : nfa'.Step nfa.nodes.size nfaClose.start pos' next pos' (.some (2 * tag + 1, pos')) := by
       apply step_close_iff.mpr
-      exact ⟨rfl, rfl, rfl, v'⟩
+      exact ⟨rfl, rfl, rfl⟩
     exact .last stepClose
   exact .more stepOpen (path.trans pathClose)
 
 theorem path_of_captures.alternateLeft {e₁ e₂} (eq : nfa.pushRegex next (.alternate e₁ e₂) = result)
-  (wf : nfa.WellFormed) (next_lt : next < nfa.nodes.size) (v : it.Valid)
+  (wf : nfa.WellFormed) (next_lt : next < nfa.nodes.size)
   (ih : ∀ {nfa : NFA} {next result}, nfa.pushRegex next e₁ = result →
     nfa.WellFormed →
     next < nfa.nodes.size →
-    ∃ update, EquivUpdate groups update ∧ result.Path nfa.nodes.size result.start it next it' update) :
-  ∃ update, EquivUpdate groups update ∧ result.Path nfa.nodes.size result.start it next it' update := by
+    ∃ update, EquivUpdate groups update ∧ result.Path nfa.nodes.size result.start pos next pos' update) :
+  ∃ update, EquivUpdate groups update ∧ result.Path nfa.nodes.size result.start pos next pos' update := by
   open Compile.ProofData Alternate in
   let pd := Alternate.intro eq
   simp [eq_result eq]
@@ -52,19 +53,19 @@ theorem path_of_captures.alternateLeft {e₁ e₂} (eq : nfa.pushRegex next (.al
   have ⟨update, eqv, path⟩ := ih (result := nfa₁) rfl wf next_lt
   exists update, eqv
 
-  have step : nfa'.Step nfa.nodes.size nfa'.start it nfa₁.start it .none := by
+  have step : nfa'.Step nfa.nodes.size nfa'.start pos nfa₁.start pos .none := by
     apply step_start_iff.mpr
-    simp [v]
+    simp
   have path := castFrom₁ path
   exact .more step path
 
 theorem path_of_captures.alternateRight {e₁ e₂} (eq : nfa.pushRegex next (.alternate e₁ e₂) = result)
-  (wf : nfa.WellFormed) (next_lt : next < nfa.nodes.size) (v : it.Valid)
+  (wf : nfa.WellFormed) (next_lt : next < nfa.nodes.size)
   (ih : ∀ {nfa : NFA} {next result}, nfa.pushRegex next e₂ = result →
     nfa.WellFormed →
     next < nfa.nodes.size →
-    ∃ update, EquivUpdate groups update ∧ result.Path nfa.nodes.size result.start it next it' update) :
-  ∃ update, EquivUpdate groups update ∧ result.Path nfa.nodes.size result.start it next it' update := by
+    ∃ update, EquivUpdate groups update ∧ result.Path nfa.nodes.size result.start pos next pos' update) :
+  ∃ update, EquivUpdate groups update ∧ result.Path nfa.nodes.size result.start pos next pos' update := by
   open Compile.ProofData Alternate in
   let pd := Alternate.intro eq
   simp [eq_result eq]
@@ -73,23 +74,23 @@ theorem path_of_captures.alternateRight {e₁ e₂} (eq : nfa.pushRegex next (.a
   have ⟨update, eqv, path⟩ := ih (result := nfa₂) rfl wf₁ (Nat.lt_trans next_lt nfa₁_property)
   exists update, eqv
 
-  have step : nfa'.Step nfa.nodes.size nfa'.start it nfa₂.start it .none := by
+  have step : nfa'.Step nfa.nodes.size nfa'.start pos nfa₂.start pos .none := by
     apply step_start_iff.mpr
-    simp [v]
+    simp
   have path := castFrom₂ (path.liftBound (Nat.le_of_lt nfa₁_property))
   exact .more step path
 
-theorem path_of_captures.concat {e₁ e₂ it it' it'' groups₁ groups₂} (eq : nfa.pushRegex next (.concat e₁ e₂) = result)
+theorem path_of_captures.concat {pos'' e₁ e₂ groups₁ groups₂} (eq : nfa.pushRegex next (.concat e₁ e₂) = result)
   (wf : nfa.WellFormed) (next_lt : next < nfa.nodes.size)
   (ih₁ : ∀ {nfa : NFA} {next result}, nfa.pushRegex next e₁ = result →
     nfa.WellFormed →
     next < nfa.nodes.size →
-    ∃ update, EquivUpdate groups₁ update ∧ result.Path nfa.nodes.size result.start it next it' update)
+    ∃ update, EquivUpdate groups₁ update ∧ result.Path nfa.nodes.size result.start pos next pos' update)
   (ih₂ : ∀ {nfa : NFA} {next result}, nfa.pushRegex next e₂ = result →
     nfa.WellFormed →
     next < nfa.nodes.size →
-    ∃ update, EquivUpdate groups₂ update ∧ result.Path nfa.nodes.size result.start it' next it'' update) :
-  ∃ update, EquivUpdate (.concat groups₁ groups₂) update ∧ result.Path nfa.nodes.size result.start it next it'' update := by
+    ∃ update, EquivUpdate groups₂ update ∧ result.Path nfa.nodes.size result.start pos' next pos'' update) :
+  ∃ update, EquivUpdate (.concat groups₁ groups₂) update ∧ result.Path nfa.nodes.size result.start pos next pos'' update := by
   open Compile.ProofData Concat in
   let pd := Concat.intro eq
   simp [pd.eq_result eq]
@@ -102,17 +103,17 @@ theorem path_of_captures.concat {e₁ e₂ it it' it'' groups₁ groups₂} (eq 
   have path₂ := castFrom₂ path₂
   exact (path₁.liftBound (Nat.le_of_lt nfa₂_property)).trans path₂
 
-theorem path_of_captures.starConcat {greedy e it it' it'' groups₁ groups₂} (eq : nfa.pushRegex next (.star greedy e) = result)
-  (wf : nfa.WellFormed) (next_lt : next < nfa.nodes.size) (v : it.Valid)
+theorem path_of_captures.starConcat {pos'' greedy e groups₁ groups₂} (eq : nfa.pushRegex next (.star greedy e) = result)
+  (wf : nfa.WellFormed) (next_lt : next < nfa.nodes.size)
   (ih₁ : ∀ {nfa : NFA} {next result}, nfa.pushRegex next e = result →
     nfa.WellFormed →
     next < nfa.nodes.size →
-    ∃ update, EquivUpdate groups₁ update ∧ result.Path nfa.nodes.size result.start it next it' update)
+    ∃ update, EquivUpdate groups₁ update ∧ result.Path nfa.nodes.size result.start pos next pos' update)
   (ih₂ : ∀ {nfa : NFA} {next result}, nfa.pushRegex next (.star greedy e) = result →
     nfa.WellFormed →
     next < nfa.nodes.size →
-    ∃ update, EquivUpdate groups₂ update ∧ result.Path nfa.nodes.size result.start it' next it'' update) :
-  ∃ update, EquivUpdate (.concat groups₁ groups₂) update ∧ result.Path nfa.nodes.size result.start it next it'' update := by
+    ∃ update, EquivUpdate groups₂ update ∧ result.Path nfa.nodes.size result.start pos' next pos'' update) :
+  ∃ update, EquivUpdate (.concat groups₁ groups₂) update ∧ result.Path nfa.nodes.size result.start pos next pos'' update := by
   open Compile.ProofData Star in
   let pd := Star.intro eq
   simp [pd.eq_result eq]
@@ -124,34 +125,34 @@ theorem path_of_captures.starConcat {greedy e it it' it'' groups₁ groups₂} (
 
   have start_eq_placeholder : nfaPlaceholder.start = nfa'.start := by
     simp [nfaPlaceholder, start_eq]
-  have path₁ : nfa'.Path nfa.nodes.size nfaExpr.start it nfa'.start it' update₁ :=
+  have path₁ : nfa'.Path nfa.nodes.size nfaExpr.start pos nfa'.start pos' update₁ :=
     start_eq_placeholder ▸ (castFromExpr path₁).liftBound (by simp [nfaPlaceholder]; exact Nat.le_succ _)
-  have step : nfa'.Step nfa.nodes.size nfa'.start it nfaExpr.start it .none :=
+  have step : nfa'.Step nfa.nodes.size nfa'.start pos nfaExpr.start pos .none :=
     if h : pd.greedy then
-      .splitLeft (j₂ := next) (by simp [start_eq]; exact Nat.le_refl _) (wf' wf next_lt).start_lt (by simp [start_eq, get_start, splitNode, h]; rfl) v
+      .splitLeft (j₂ := next) (by simp [start_eq]; exact Nat.le_refl _) (wf' wf next_lt).start_lt (by simp [start_eq, get_start, splitNode, h]; rfl)
     else
-      .splitRight (j₁ := next) (by simp [start_eq]; exact Nat.le_refl _) (wf' wf next_lt).start_lt (by simp [start_eq, get_start, splitNode, h]; rfl) v
+      .splitRight (j₁ := next) (by simp [start_eq]; exact Nat.le_refl _) (wf' wf next_lt).start_lt (by simp [start_eq, get_start, splitNode, h]; rfl)
 
   exact (Path.more step path₁).trans path₂
 
 theorem path_of_captures (eq : nfa.pushRegex next e = result)
   (wf : nfa.WellFormed) (next_lt : next < nfa.nodes.size)
-  (c : e.Captures it it' groups) :
-  ∃ update, EquivUpdate groups update ∧ result.Path nfa.nodes.size result.start it next it' update := by
+  (c : e.Captures pos pos' groups) :
+  ∃ update, EquivUpdate groups update ∧ result.Path nfa.nodes.size result.start pos next pos' update := by
   open Compile.ProofData in
   induction c generalizing nfa next result with
-  | @char it l c r vf =>
+  | char ne hc =>
     let pd := Char.intro eq
     exists [], .empty
     simp [pd.eq_result eq]
     apply (pd.path_start_iff next_lt).mpr
-    exists l, r
-  | @sparse it l c r cs vf mem =>
+    exact ⟨rfl, rfl, ne, rfl, hc⟩
+  | sparse ne mem =>
     let pd := Classes.intro eq
     exists [], .empty
     simp [pd.eq_result eq]
     apply (pd.path_start_iff next_lt).mpr
-    exists l, c, r
+    exact ⟨rfl, rfl, ne, rfl, mem⟩
   | epsilon =>
     let pd := Epsilon.intro eq
     exists [], .empty
@@ -164,24 +165,23 @@ theorem path_of_captures (eq : nfa.pushRegex next e = result)
     simp [pd.eq_result eq]
     apply (pd.path_start_iff next_lt).mpr
     trivial
-  | group c ih => exact path_of_captures.group eq wf next_lt c.validL c.validR ih
-  | alternateLeft c ih => exact path_of_captures.alternateLeft eq wf next_lt c.validL ih
-  | alternateRight c ih => exact path_of_captures.alternateRight eq wf next_lt c.validL ih
+  | group c ih => exact path_of_captures.group eq wf next_lt ih
+  | alternateLeft c ih => exact path_of_captures.alternateLeft eq wf next_lt ih
+  | alternateRight c ih => exact path_of_captures.alternateRight eq wf next_lt ih
   | concat _ _ ih₁ ih₂ => exact path_of_captures.concat eq wf next_lt ih₁ ih₂
-  | @starEpsilon it greedy e v =>
+  | @starEpsilon pos _ _ =>
     let pd := Star.intro eq
     exists [], .empty
     simp [pd.eq_result eq]
 
-    have step : nfa'.Step nfa.nodes.size nfa'.start it next it .none := by
+    have step : nfa'.Step nfa.nodes.size nfa'.start pos next pos .none := by
       apply (pd.step_start_iff).mpr
-      simp
-      exact ⟨.inr rfl, v⟩
+      exact ⟨.inr rfl, rfl, rfl⟩
     exact .last step
-  | starConcat c₁ _ ih₁ ih₂ => exact path_of_captures.starConcat eq wf next_lt c₁.validL ih₁ ih₂
+  | starConcat c₁ _ ih₁ ih₂ => exact path_of_captures.starConcat eq wf next_lt ih₁ ih₂
 
-theorem path_of_captures_compile (eq : compile e = nfa) (c : e.Captures it it' groups) :
-  ∃ update, EquivUpdate groups update ∧ nfa.Path 1 nfa.start it 0 it' update := by
+theorem path_of_captures_compile (eq : compile e = nfa) (c : e.Captures pos pos' groups) :
+  ∃ update, EquivUpdate groups update ∧ nfa.Path 1 nfa.start pos 0 pos' update := by
   simp [←eq, compile]
   exact path_of_captures rfl done_WellFormed (by decide) c
 
